% -*- mode: context; -*-
\chapter{Determinants}
\startitemize[n, 1*broad]
\item Let $\Delta = \startdeterminant\NC  4 \NC 9 \NC 7\NR\NC 3 \NC 5 \NC 7\NR\NC 5 \NC 4 \NC
  5\NR\stopdeterminant$

  $\Delta = \startdeterminant\NC  1 \NC 4 \NC 0\NR\NC 3 \NC 5 \NC 7\NR\NC 5 \NC 4 \NC
  5\NR\stopdeterminant[R_1\rightarrow R_1 - R_2] = \startdeterminant\NC  1 \NC 4 \NC 0\NR\NC 0 \NC -7 \NC
  7\NR\NC 0 \NC -16 \NC 5\NR\stopdeterminant[R_2\rightarrow R_2 - 3R_1$ and $R_3\rightarrow R_3 - 5R_1]$

  $= 1(-35 + 112) = 77$.
\item Let $\Delta = \startdeterminant\NC  1 \NC a\NC a^2\NR\NC 1 \NC b \NC b^2\NR\NC 1 \NC c \NC
  c^2\NR\stopdeterminant$

  $= \startdeterminant\NC  0 \NC a - b\NC a^2 - b^2\NR\NC 0 \NC b - c \NC b^2 - c^2\NR\NC 1 \NC c \NC
  c^2\NR\stopdeterminant[R_1\rightarrow R_1 - R_2; R_2\rightarrow R_2 - R_3]$

  $= (a - b)(b - c)\startdeterminant\NC  0 \NC 1\NC a + b\NR\NC 0 \NC 1 \NC b + c\NR\NC 1 \NC c \NC
  c^2\NR\stopdeterminant = (a - b)(b - c)(b + c - a - b) = (a - b)(b - c)(c - a)$.
\item Let $a = 2, b = 3, c = 4$ then $\Delta = \startdeterminant\NC  1 \NC 2\NC 4\NR\NC 1 \NC 3 \NC 9\NR\NC
  1 \NC 4 \NC 16\NR\stopdeterminant = \startdeterminant\NC  1 \NC a\NC a^2\NR\NC 1 \NC b \NC b^2\NR\NC 1 \NC
  c \NC c^2\NR\stopdeterminant$

  We can solve this like previous problem which gives us $\Delta = (2 - 3)(3 - 4)(4 - 2) = 2$.
\item Let $\Delta = \startdeterminant\NC  4 \NC 9 \NC 2\NR\NC 3 \NC 5 \NC 7\NR\NC 8 \NC 1 \NC
  6\NR\stopdeterminant =\startdeterminant\NC  1 \NC 4 \NC -5\NR\NC 3 \NC 5 \NC 7\NR\NC 8 \NC 1 \NC
  6\NR\stopdeterminant[R_1\rightarrow R_1 - R_2]$

  $= \startdeterminant\NC  1 \NC 4 \NC -5\NR\NC 0 \NC -7 \NC 22\NR\NC 0 \NC -31 \NC
  46\NR\stopdeterminant[R_2\rightarrow R_2 - 3R_1; R_3\rightarrow R_3 - 5R_1]$

  $= (-322 + 682) = 360$.
\item Let $\Delta = \startdeterminant\NC  18 \NC 1 \NC 17\NR\NC 22 \NC 3 \NC 19\NR\NC 26 \NC 5 \NC
  21\NR\stopdeterminant = \startdeterminant\NC  18 \NC 1 \NC 17\NR\NC 4 \NC 2 \NC 2\NR\NC 4 \NC 2 \NC
  2\NR\stopdeterminant[R_3\rightarrow R_3 - R_2; R_2\rightarrow R_2 - R_1]$

  $= 0$(bceuase two rows are identical).
\item Let $\Delta = \startdeterminant\NC  4 \NC 9 \NC 7\NR\NC 3 \NC 5 \NC 7\NR\NC 5 \NC 4 \NC
  5\NR\stopdeterminant = \startdeterminant\NC  1 \NC 4 \NC 0\NR\NC 3 \NC 5 \NC 7\NR\NC 5 \NC 4 \NC
  5\NR\stopdeterminant[R_1\rightarrow R_2 - R_1]$

  $= \startdeterminant\NC 1 \NC 4 \NC 0\NR\NC 0 \NC -7 \NC 7\NR\NC 0 \NC -16 \NC
  5\NR\stopdeterminant[R_2\rightarrow R_2 - 3R_1;R_3\rightarrow R_3 - R_1]$

  $= (-35 + 112) = 77$.
\item $\Delta = \startdeterminant\NC 1 \NC 4\NC 9\NR\NC 3\NC 5\NC 7\NR\NC 5 \NC 7\NC
  9\NR\stopdeterminant[R_3\rightarrow R_3 - R_2; R_2\rightarrow R_2 - R_1]= \startdeterminant\NC 1\NC
  4\NC 9\NR\NC 3\NC 5\NC 7\NR\NC 2\NC 2\NC
  2\NR\stopdeterminant[R_3\rightarrow R_3 - R_2]$

  $=\startdeterminant\NC 1\NC 3\NC 5\NR\NC 3\NC 2\NC 2\NR\NC 2\NC 0\NC
  0\NR\stopdeterminant[C_3\rightarrow C_3 - C_2; C_2\rightarrow C_2 - C_1] = 2(6 - 10) = -8$.
\item Let $\Delta = \startdeterminant\NC  a \NC b \NC c\NR\NC b \NC c \NC a\NR\NC c \NC a \NC
  b\NR\stopdeterminant = \startdeterminant\NC  a + b + c \NC b \NC c\NR\NC b + c + a \NC c \NC a\NR\NC c + a
  + b\NC a \NC b\NR\stopdeterminant[C_1\rightarrow C_1 + C_2 + C_3]$

  $= (a + b + c)\startdeterminant\NC 1 \NC b \NC c\NR\NC 1 \NC c \NC a\NR\NC 1 \NC a \NC
  b\NR\stopdeterminant = (a + b + c)\startdeterminant\NC  1 \NC b \NC c\NR\NC 0 \NC c - b \NC a - c\NR\NC 0
  \NC a - b \NC b - c\NR\stopdeterminant[R_2\rightarrow R_2 - R_1; R_3\rightarrow R_3 - R_1]$

  $= (a + b + c)[(c - b)(b - c) - (a - b)(a - c)] = (a + b + c)(ab + bc + ca - a^2 - b^2 - c^2) =
  -\frac{1}{2}(a + b + c)[(a - b)^2 + (b - c)^2 + (c - a)^2]$

  Given that $a, b, c$ are positive so $a + b + c > 0$ and since $a, b, c$ are unequal so $(a - b)^2 + (b -
  c)^2 + (c - a)^2 > 0$. Thus, $\Delta < 0$.
\item Let $\Delta = \startdeterminant\NC  b + c\NC a + b \NC a\NR\NC c + a \NC b + c \NC b\NR\NC a + b \NC c
  + a \NC c\NR\stopdeterminant = \startdeterminant\NC  a + b + c\NC a + b \NC a\NR\NC b + c + a \NC b + c
  \NC b\NR\NC a + b + c \NC c + a \NC c\NR\stopdeterminant[C_1\rightarrow C_1 + C_3]$

  $= (a + b + c)\startdeterminant\NC 1\NC a + b \NC a\NR\NC 1 \NC b + c \NC b\NR\NC 1 \NC c + a \NC
  c\NR\stopdeterminant = (a + b + c)\startdeterminant\NC 1\NC a + b \NC a\NR\NC 0 \NC c - a \NC b - a\NR\NC
  0 \NC c - b \NC c - a\NR\stopdeterminant[R_2\rightarrow R_2 - R_1; R_3\rightarrow R_3 - R_1]$

  $= (a + b + c)[(c - a)^2 - (c - b)(b - a)] = (a + b + c)(a^2 + b^2 + c^2 - ab - bc - ca) = a^3 + b^3 + c^3
  - 3abc$.
\item $\Delta = \startdeterminant\NC  1 + a_1 + a_2 + a_3\NC a_2 \NC a_3\NR\NC 1 + a_1 + a_2 + a_3 \NC 1+
  a_2 \NC a_3\NR\NC 1 + a_1 + a_2 + a_3 \NC a_2 \NC 1 + a_3\NR\stopdeterminant[C_1\rightarrow C_1 + C_2 +
  C_3]$

  $= (1 + a_1 + a_2 + a_3)\startdeterminant\NC  1\NC a_2 \NC a_3\NR\NC 1\NC 1 + a_2 \NC a_3\NR\NC 1\NC a_2
  \NC 1 + a_3\NR\stopdeterminant = (1 + a_1 + a_2 + a_3)\startdeterminant\NC  0\NC -1 \NC 0\NR\NC 0\NC 1 \NC
  -1\NR\NC 1\NC a_2 \NC 1 + a_3\NR\stopdeterminant[R_1\rightarrow R_1 - R_2; R_2\rightarrow R_2 - R_3]$

  $= (1 + a_1 + a_2 + a_3)\startdeterminant\NC -1 \NC 0\NR\NC 1\NC -1\NR\stopdeterminant = 1 + a_1 + a_2
  + a_3$.
\item $\Delta = \startdeterminant\NC  2a + 2b + 2c \NC a \NC b\NR\NC 2a + 2b + 2c \NC b + c + 2a \NC b\NR\NC
  2a + 2b + 2c \NC a \NC c + a + 2b\NR\stopdeterminant[C_1\rightarrow C_1 + C_2 + C_3]$

  $= 2(a + b + c)\startdeterminant\NC  1 \NC a \NC b\NR\NC 1 \NC b + c + 2a \NC b\NR\NC 1 \NC a \NC c + a +
  2b\NR\stopdeterminant$

  $= 2(a + b + c)\startdeterminant\NC  0 \NC -(a + b + c) \NC 0\NR\NC 0 \NC b + c + a
  \NC -(a + b + c)\NR\NC 1 \NC a \NC c + a + 2b\NR\stopdeterminant [R_1\rightarrow R_1 - R_2; R_2\rightarrow
  R_2 - R_3]$

  $= 2(a + b + c)^3\startdeterminant\NC 0\NC -1\NC 0\NR\NC 0\NC 1\NC -1\NR\NC 1\NC a\NC c + a +
  2b\NR\stopdeterminant$(taking $a + b + c$ common from first and second row)

  $= 2(a + b + c)^3[-1.-1 - 1.0] = 2(a + b + c)^3$.
\item $\Delta = \startdeterminant\NC 2a\NC 2b \NC a - b - c\NR\NC 2b\NC 2c\NC b - c - a\NR\NC 2c\NC 2a\NC
  c - a - b\NR\stopdeterminant[C_1\rightarrow C_1 + C_2; C_2\rightarrow C_2 - C_3]$

  $= 4\startdeterminant\NC a\NC b \NC a - b - c\NR\NC b\NC c\NC b - c - a\NR\NC c\NC a\NC
  c - a - b\NR\stopdeterminant$

  $= 4\startdeterminant\NC a \NC b\NC c\NR\NC b\NC c\NC a\NR\NC c\NC a\NC b\NR\stopdeterminant = 4(a + b
  + c)(a^2 + b^2 + c^2 - ab - bc - ca) = 4(a^3 + b^3 + c^3 - 3abc)$.
\item $\Delta = \startdeterminant\NC  a + b + c \NC a + b + c \NC a + b + c\NR\NC 2b \NC b - c - a\NR\NC 2c
  \NC 2c \NC c - a - b\NR\stopdeterminant[R_1\rightarrow R_1 + R_2 + R_3]$

  $= (a + b + c)\startdeterminant\NC 1 \NC 1 \NC 1\NR\NC 2b \NC b - c - a\NC 2b\NR\NC 2c \NC 2c\NC c - a - b
  \NR\stopdeterminant$

  $= (a + b + c)\startdeterminant\NC 1 \NC 0 \NC 0\NR\NC 2b \NC -b - c - a\NC 0\NR\NC 2c \NC 0\NC -c - a - b
  \NR\stopdeterminant[C_1\rightarrow C_2 - C_1; C_3\rightarrow C_3 - C_1]$

  $= (a + b + c)\startdeterminant\NC -b - c - a\NC 0\NR\NC 0 \NC -c - a - b\NR\stopdeterminant = (a + b +
  c)^3$.
\item $\Delta = \frac{1}{x.y.z}\startdeterminant\NC x^2\NC y^2\NC z^2\NR\NC x^3\NC y^3\NC z^3\NR\NC xyz\NC
  xyz\NC xyz\NR\stopdeterminant[C_1\rightarrow xC_1; C_2\rightarrow yC_2; C_3\rightarrow zC_3]$

  $= \frac{xyz}{xyz}\startdeterminant\NC x^2\NC y^2\NC z^2\NR\NC x^3\NC y^3\NC z^3\NR\NC 1\NC
  1\NC 1\NR\stopdeterminant = \startdeterminant\NC1 \NC 1\NC 1\NR\NC x^2 \NC y^2\NC z^2\NR\NC x^3 \NC y^3\NC
  z^3\NR\stopdeterminant$(exchanging rows twice)

  $= \startdeterminant\NC 1\NC 0\NC\NR\NC x^2 \NC y^2-x^2 \NC z^2 - x^2\NR\NC x^3\NC y^3 - x^3\NC z^3 -
  x^3\NR\stopdeterminant[C_2\rightarrow C_2 - C_1; C_3\rightarrow C_3 - C_1]$

  $= \startdeterminant\NC(y - x)(y + x)\NC (z - x)(z + x)\NR\NC (y - x)(y^2 + xy + x^2)\NC (z - x)(z^2 + zx
  + x^2)\NR\stopdeterminant$

  $= (y - x)(z - x)\startdeterminant\NC y + x\NC z + x\NR\NC y^2 + xy + y^2\NC z^2 + zx +
  x^2\NR\stopdeterminant$

  $= (y - x)(z - x)\startdeterminant\NC y + x\NC z - y\NR\NC y^2 + yx + x^2 \NC (z^2 - y^2) + zx -
  zy\NR\stopdeterminant[C_2\rightarrow C_2 - C_1]$

  $= (y - x)(z - x)(z - y)\startdeterminant\NC y + z\NC 1\NR\NC y^2 + xy + x^2 \NC x + y +
  z\NR\stopdeterminant$

  $= (y - x)(z - x)(z - y)[(y + x)(x + y + z) - y^2 - xy - x^2] = (x - y)(y - z)(z - x)(xy + yz + zx)$.
\item $\Delta = \frac{1}{abc}\startdeterminant\NC  a(a^2 + 1) \NC ab^2 \NC ac^2\NR\NC a^2b \NC b(b^2 + 1)
  \NC bc^2\NR\NC a^2c \NC b^2c \NC c(c^2 + 1)\NR\stopdeterminant[C_1\rightarrow aC_1; C_2\rightarrow bC_2;
  C_3\rightarrow cC_3]$

  $= \frac{abc}{abc}\startdeterminant\NC a^2 + 1\NC b^2\NC c^2\NR\NC a^2 \NC b^2 + 1\NC c^2\NR\NC a^2 \NC
  b^2\NC c^2 + 1\NR\stopdeterminant$

  $= \startdeterminant\NC 1 + a^2 + b^2 + c^2\NC b^2\NC c^2\NR\NC 1 + a^2 + b^2 + c^2 \NC b^2 + 1\NC
  c^2\NR\NC 1 + a^2 + b^2 + c^2 \NC b^2\NC c^2 + 1\NR\stopdeterminant[C_1\rightarrow C_1 + C_2 + C_3]$

  $= (1 + a^2 + b^2 + c^2)\startdeterminant\NC 1\NC b^2\NC c^2\NR\NC 1\NC b^2 + 1\NC c^2\NR\NC 1\NC b^2\NC
  c^2 + 1\NR\stopdeterminant$

  $= (1 + a^2 + b^2 + c^2)\startdeterminant\NC 1 \NC b^2\NC c^2\NR\NC 0 \NC 1\NC 0\NR\NC 0 \NC 0\NC
  1\NR\stopdeterminant[R_2\rightarrow R_2 - R_1; R_3\rightarrow R_3 - R_1]$

  $= (1 + a^2 + b^2 + c^2)\startdeterminant\NC1 \NC 0\NR\NC 0\NC 1\NR\stopdeterminant = 1 + a^2 + b^2 +
  c^2$.
\item $\Delta = a_1a_2a_3\startdeterminant\NC \frac{1}{a_1} + 1\NC \frac{1}{a_2}\NC \frac{1}{a_3}\NR\NC
  \frac{1}{a_1}\NC \frac{1}{a_2} + 1\NC \frac{1}{a_3}\NR\NC \frac{1}{a_1}\NC \frac{1}{a_2} \NC \frac{1}{a_3}
  + 1\NR\stopdeterminant[C_1\rightarrow \frac{C_1}{a_1}; C_2\rightarrow \frac{C_2}{a_2}; C_3\rightarrow
  \frac{C_3}{a_3}]$

  $= a_1a_2a_2\startdeterminant\NC 1 + \frac{1}{a_1} + \frac{1}{a_2} + \frac{1}{a_3} \NC \frac{1}{a_2}\NC
  \frac{1}{a_3}\NR\NC 1 + \frac{1}{a_1} + \frac{1}{a_2} + \frac{1}{a_3}\NC \frac{1}{a_2} + 1\NC
  \frac{1}{a_3}\NR\NC 1 + \frac{1}{a_1} + \frac{1}{a_2} + \frac{1}{a_3}\NC \frac{1}{a_2}\NC \frac{1}{a_3} +
  1\NR\stopdeterminant[C_1\rightarrow C_1 + C_2 + C_3]$

  $= a_1a_2a_3\left(1 + \frac{1}{a_1} + \frac{1}{a_2} + \frac{1}{a_3}\right)\startdeterminant\NC 1 \NC
  \frac{1}{a_2}\NC \frac{1}{a_3}\NR\NC 1\NC \frac{1}{a_2} + 1\NC \frac{1}{a_3}\NR\NC 1\NC \frac{1}{a_2}\NC
  \frac{1}{a_3} + 1\NR\stopdeterminant$

  $= a_1a_2a_3\left(1 + \frac{1}{a_1} + \frac{1}{a_2} + \frac{1}{a_3}\right)\startdeterminant\NC1
  \NC\frac{1}{a_2}\NC \frac{1}{a_3}\NR\NC 0\NC 1\NC 0\NR\NC 0\NC 0\NC 1\NR\stopdeterminant[R_2\rightarrow
  R_2 - R_1; R_3\rightarrow R_3 - R_1]$

  $= a_1a_2a_3\left(1 + \frac{1}{a_1} + \frac{1}{a_2} + \frac{1}{a_3}\right)$.
\item $\Delta = \startdeterminant\NC  x \NC x^2 \NC 1 + x^3\NR\NC y \NC y^2 \NC 1 + y^3\NR\NC z \NC z^2 \NC
  1 + z^3\NR\stopdeterminant = \startdeterminant\NC  x \NC x^2 \NC x^3\NR\NC y \NC y^2 \NC y^3\NR\NC z \NC
  z^2 \NC z^3\NR\stopdeterminant + \startdeterminant\NC  x \NC x^2 \NC 1\NR\NC y \NC y^2 \NC 1\NR\NC z \NC
  z^2 \NC 1\NR\stopdeterminant$

  $= xyz\startdeterminant\NC 1\NC x\NC x^2\NR\NC 1\NC y\NC y^2\NR\NC 1\NC z\NC z^2\NR\stopdeterminant +
  \startdeterminant\NC 1\NC x\NC x^2\NR\NC 1\NC y\NC y^2\NR\NC 1\NC z\NC z^2\NR\stopdeterminant$(by
  exchanging two columns)

  $= (1 + xyz)\startdeterminant\NC 1\NC x\NC x^2\NR\NC 1\NC y\NC y^2\NR\NC 1\NC z\NC z^2\NR\stopdeterminant
  = (1 + xyz)(x - y)(y - z)(z - x)$(from the value of a circular determinant)

  $\Delta = 0 \Rightarrow 1 + xyz = 0[\because x\neq y;y\neq z;z\neq x]\Rightarrow xyz = -1$.
\item $\Delta = \startdeterminant\NC 0 \NC -2c \NC -2b\NR\NC b \NC c + a\NC b\NR\NC a\NC c\NC a +
  b\NR\stopdeterminant[R_1\rightarrow R_1 - R_2 - R_3]$

  $= \frac{1}{c}\startdeterminant\NC 0 \NC -2c\NC -2b\NR\NC 0\NC c(c + a - b)\NC b(c - a - b)\NR\NC c\NC
  c\NC a + b\NR\stopdeterminant[R_2\rightarrow cR_2 - bR_3]$

  $= \frac{1}{c}c(-2bc)[c - a - b - (c + a - b)] = -2bc.-2a = 4abc$.
\item $\Delta = \startdeterminant\NC(b + c)^2 - a^2\NC 0\NC a^2\NR\NC b^2 - (c + a)^2\NC (c + a)^2 - b^2\NC
  b^2\NR\NC 0\NC c^2 - (a + b)^2 \NC (a + b)^2\NR\stopdeterminant[C_1\rightarrow C_1 - C_2; C_2\rightarrow
  C_2 - C_3]$

  $= (a + b + c)^2\startdeterminant\NC b + c - a\NC 0\NC a^2\NR\NC b+ c - a\NC c + a - b\NC b^2\NR\NC 0 \NC
  c - a - b\NC (a + b)^2\NR\stopdeterminant$

  $= (a + b + c)^2\startdeterminant\NC b + c - a\NC 0\NC a^2\NR\NC b+ c - a\NC c + a - b\NC b^2\NR\NC 2a -
  2b\NC -2a\NC 2ab\NR\stopdeterminant[R_3\rightarrow R_3 - R_1 - R_2]$

  $= (a + b + c)^2\startdeterminant\NC b + c - a\NC 0\NC a^2\NR\NC 0\NC c + a - b\NC b^2\NR\NC -2b\NC -2a\NC
  2ab\NR\stopdeterminant[C_1\rightarrow C_1 + C_2]$

  $= \frac{(a + b + c)^2}{ab}\startdeterminant\NC a(b + c)\NC a^2\NC a^2\NR\NC b^2\NC b(c + a) \NC b^2\NR\NC
  0\NC 0\NC 2ab\NR\stopdeterminant[C_1\rightarrow aC_1 + C_3; C_2\rightarrow bC_2 + C_3]$

  $= \frac{(a + b + c)^2}{ab}.ab.2ab\startdeterminant\NC b + c\NC a\NC a\NR\NC b\NC c + a\NC b\NR\NC 0\NC
  0\NC 1\NR\stopdeterminant$

  $= 2ab(a + b + c)^2[(b + c)(c + a) - ab] = 2abc(a + b + c)^3$.
\item $\Delta = \startdeterminant\NC 15 - x\NC 1\NC 10\NR\NC -4 -2x\NC 0\NC 6\NR\NC -8\NC 0\NC
  3\NR\stopdeterminant = 0[R_2\rightarrow R_2 - R_1; R_3\rightarrow R_3 - R_1]$

  $\Rightarrow (12 + 6x - 48) = 0 \Rightarrow x = 6$.
\item $\Delta = \startdeterminant\NC a + b + c - x\NC c\NC b\NR\NC a + b + c - x\NC b - x\NC a\NR\NC a + b +
  c - x\NC a\NC c - x\NR\stopdeterminant = 0[C_1\rightarrow C_1 + C_2 + C_3]$

  $\Rightarrow \startdeterminant\NC -x\NC c\NC b\NR\NC -x\NC b - x\NC a\NR\NC -x\NC a\NC c -
  x\NR\stopdeterminant = 0[\because a + b + c = 0]$

  $\Rightarrow (-x)\startdeterminant\NC 1\NC c\NC b\NR\NC 1\NC b - x\NC a\NR\NC 1\NC a\NC c -
  x\NR\stopdeterminant = 0$

  $\Rightarrow \startdeterminant\NC1 \NC c\NC b\NR\NC 0\NC b - c - x\NC a - b\NR\NC 0\NC a- c\NC c - b -
  x\NR\stopdeterminant = 0[R_2\rightarrow R_2 - R_1; R_3\rightarrow R_3 - R_1]$

  $\Rightarrow x[(b - c - x)(c - b - x) - (a - c)(a - b)] = 0 \Rightarrow x(x^2 - a^2 - b^2 - c^2 + ab + bc
  + ca) = 0$

  $\Rightarrow x = 0; x^2 = (a^2 + b^2 + c^2) - \frac{1}{2}[(a + b + c)^2 - (a^2 + b^2 + c^2)] =
  \frac{3}{2}(a^2 + b^2 + c^2)[\because a + b + c = 0]\Rightarrow x = \pm\sqrt{\frac{3}{2}(a^2 + b^2 +
    c^2)}$.
\item $D_1 = \startdeterminant\NC  a \NC b \NC c\NR\NC d \NC e \NC f\NR\NC g \NC h \NC k\NR\stopdeterminant
  = \startdeterminant\NC  a \NC b \NC c\NR\NC tx \NC ty \NC tc\NR\NC g \NC h \NC k\NR\stopdeterminant$

  $= t\startdeterminant\NC  a \NC b \NC c\NR\NC x \NC y \NC z\NR\NC g \NC h \NC k\NR\stopdeterminant =
  t\startdeterminant\NC  a \NC x \NC g\NR\NC b \NC y \NC h\NR\NC c \NC z \NC k\NR\stopdeterminant$(changing
  rows into corresponding columns)

  $= -t\startdeterminant\NC a\NC g \NC x\NR\NC b \NC h \NC y\NR\NC c \NC k \NC z\NR\stopdeterminant =
  -tD_2$.
\item $\startdeterminant\NC  a \NC bc \NC abc \NR\NC b \NC ca \NC abc\NR\NC c \NC ab \NC
  abc\NR\stopdeterminant = \frac{1}{a^2b^2c^2}\startdeterminant\NC a^3\NC a^2bc\NC a^3bc\NR\NC b^3\NC
  ab^2c\NC ab^3c\NR\NC c^3\NC abc^2\NC abc^3\NR\stopdeterminant[R_1\rightarrow a^2R_1; R_2\rightarrow
  b^2R_2; R_3\rightarrow c^2R_3]$

  $= \frac{abc.abc}{a^2b^2c^2}\startdeterminant\NC a^3\NC a\NC a^2\NR\NC b^3\NC b\NC b^2\NR\NC c^3\NC c\NC
  c^2\NR\stopdeterminant$

  $= \startdeterminant\NC  a \NC a^2 \NC a^3\NR\NC b \NC b^2 \NC b^3\NR\NC c \NC c^2 \NC
  c^3\NR\stopdeterminant$(exchanging columns twice).
\stopitemize